haskell/Optics/Optics/Nat.hs
@@ -9,59 +9,14 @@
 
 module  Optics.Nat
     (   Nat         (..)
-    ,   SNat
-    ,   KnownNat    (..)
-    ,   Sing        (..)
-    ,   natVal
-    ,   fromSNat
     )   where
-
-import Prelude      hiding (toInteger)
-
-import Optics.Singleton
 
 data Nat = Z | S Nat
     deriving (Eq)
 
-{-
--- SNat 'Z has only one instance
--- SNat ('S 'Z) has only one instance
--- ...
-data SNat (n :: Nat) :: Type where
-    SZ :: SNat 'Z
-    SS :: forall (n :: Nat) . SNat n -> SNat ('S n)
--}
-
-data instance Sing (a :: Nat) where
-    SZ :: Sing 'Z
-    SS :: Sing n -> Sing ('S n)
-
-type SNat (a :: Nat) = Sing a
-
-
-class KnownNat (n :: Nat) where
-    natSing :: SNat n
-
-instance KnownNat 'Z where
-    natSing = SZ
-
-instance (KnownNat n) => KnownNat ('S n) where
-    natSing = SS natSing
-
-natVal :: forall n proxy . KnownNat n => proxy n -> Nat
-natVal _ = fromSNat (natSing @ n)
-
-toInteger :: Nat -> Integer
-toInteger Z = 0
-toInteger (S n) = 1 + toInteger n
-
 instance Show Nat where
-    show = show . toInteger
+    show = show . fromNat
 
-fromSNat :: SNat n -> Nat
-fromSNat SZ     = Z
-fromSNat (SS n) = S (fromSNat n)
-
-instance Show (SNat n) where
-    show = show . fromSNat
-
+fromNat :: Nat -> Integer
+fromNat Z = 0
+fromNat (S n) = 1 + fromNat n
