haskell/Optics/Optics/Singleton.hs
@@ -1,11 +1,22 @@
+{-# LANGUAGE GADTs                  #-}
+{-# LANGUAGE DataKinds              #-}
 {-# LANGUAGE PolyKinds              #-}
 {-# LANGUAGE TypeFamilies           #-}
 {-# LANGUAGE KindSignatures         #-}
+{-# LANGUAGE TypeApplications       #-}
+{-# LANGUAGE FlexibleInstances      #-}
+{-# LANGUAGE ScopedTypeVariables    #-}
 
 module  Optics.Singleton
-    (   Sing 
-    ,   SingE   (..)  
+    (   Sing        (..)
+    ,   SingE       (..)  
+    ,   SBool
+    ,   SNat
+    ,   KnownNat    (..)
+    ,   natVal
     )   where
+
+import Optics.Nat
 
 data family Sing (a :: k) 
 
@@ -13,9 +24,48 @@ data family Sing (a :: k)
 instance Eq (Sing a) where
     (==) _ _ = True
 
-
 class SingE (a :: k) where
     type Demote a
     fromSing :: Sing a -> Demote a
 
+-- SBool
+type SBool (a :: Bool) = Sing a
 
+data instance Sing (a :: Bool) where
+    STrue  :: Sing 'True
+    SFalse :: Sing 'False 
+
+instance Show (SBool a) where
+    show = show . fromSing
+
+instance SingE (a :: Bool) where
+    type Demote a = Bool
+    fromSing STrue  = True
+    fromSing SFalse = False
+
+--SNat
+type SNat (a :: Nat) = Sing a
+
+data instance Sing (a :: Nat) where
+    SZ :: Sing 'Z
+    SS :: Sing n -> Sing ('S n)
+
+instance Show (SNat n) where
+    show = show . fromSing
+
+instance SingE (n :: Nat) where
+    type Demote a = Nat
+    fromSing SZ = Z
+    fromSing (SS n) = S (fromSing n)
+
+class KnownNat (n :: Nat) where
+    natSing :: SNat n
+
+instance KnownNat 'Z where
+    natSing = SZ
+
+instance (KnownNat n) => KnownNat ('S n) where
+    natSing = SS natSing
+
+natVal :: forall n proxy . KnownNat n => proxy n -> Nat
+natVal _ = fromSing (natSing @ n)
