haskell/Optics/Optics/Test/Nat.hs
@@ -8,13 +8,5 @@ import Optics.Nat
 
 specNat :: Spec
 specNat = describe "Testing Nat..." $ do
-    specFromSNatZ
-    specFromSNatS
+    return ()
 
-specFromSNatZ :: Spec
-specFromSNatZ = it "Checked (fromSNat SZ)" $ do
-    fromSNat SZ `shouldBe` Z
-
-specFromSNatS :: Spec
-specFromSNatS = it "Checked (fromSNat (SS SZ))" $ do
-    fromSNat (SS SZ) `shouldBe` (S Z)
