haskell/Optics/Optics/Test/Singleton.hs
@@ -1,0 +1,34 @@
+module  Optics.Test.Singleton
+    (   specSingleton
+    )   where
+
+import Test.Hspec
+
+
+import Optics.Nat
+import Optics.Singleton
+
+specSingleton :: Spec
+specSingleton = describe "Testing Singleton..." $ do
+    specSBoolTrue
+    specSBoolFalse
+    specFromSNatZ
+    specFromSNatS
+
+
+specSBoolTrue :: Spec 
+specSBoolTrue = it "Checked fromSing STrue" $ do
+    fromSing STrue `shouldBe` True
+
+
+specSBoolFalse :: Spec 
+specSBoolFalse = it "Checked fromSing SFalse" $ do
+    fromSing SFalse `shouldBe` False
+
+specFromSNatZ :: Spec
+specFromSNatZ = it "Checked (fromSNat SZ)" $ do
+    fromSing SZ `shouldBe` Z
+
+specFromSNatS :: Spec
+specFromSNatS = it "Checked (fromSNat (SS SZ))" $ do
+    fromSing (SS SZ) `shouldBe` (S Z)
