coq/set/Core/Syntax.v
@@ -1,3 +1,7 @@
+Require Import List.
+
+Require Import Core.Nat.
+
 Inductive Formula : Type :=
 | Bot  : Formula
 | Elem : nat -> nat -> Formula
@@ -5,14 +9,55 @@ Inductive Formula : Type :=
 | All  : nat -> Formula -> Formula
 .
 
+Fixpoint fresh (m:nat) (n:nat) : nat :=
+    match eq_nat_dec 0 m, eq_nat_dec 0 n with
+    | right _, right _  => 0 
+    | left  _, left  _  => 1
+    | left  _, right _  =>          (* m = 0 so cannot use 0 *)
+        match eq_nat_dec 1 n with
+        | left  _       => 2        (* n = 1 so cannot use 1 *)
+        | right _       => 1 
+        end
+    | right _, left  _  =>          (* n = 0 so cannot use 0 *) 
+        match eq_nat_dec 1 m with
+        | left  _       => 2        (* m = 1 so cannot use 1 *)
+        | right _       => 1      
+        end
+    end.
+
 Definition Not (p:Formula)          :Formula := Imp p Bot.
 Definition Or  (p q:Formula)        :Formula := Imp (Not p) q.
 Definition And (p q:Formula)        :Formula := Not (Or (Not p) (Not q)).
 Definition Exi  (n:nat) (p:Formula) :Formula := Not (All n (Not p)).
 Definition Iff (p q:Formula)        :Formula := And (Imp p q) (Imp q p).
-Definition Sub (m n:nat)            :Formula := All 0 (Imp (Elem 0 m) (Elem 0 n)).
-Definition Equ (m n:nat)            :Formula := And
-    (All 0 (Iff (Elem 0 m) (Elem 0 n)))
-    (All 0 (Iff (Elem m 0) (Elem n 0))).
 
+Definition Sub (m n:nat) : Formula := 
+    let x := fresh m n in
+        All x (Imp (Elem x m) (Elem x n)).
+
+Definition Equ (m n:nat) : Formula := 
+    let x := fresh m n in And
+        (All x (Iff (Elem x m) (Elem x n)))
+        (All x (Iff (Elem m x) (Elem n x))).
+
+Lemma checkFresh00 : fresh 0 0 = 1.
+Proof. reflexivity. Qed.
+
+Lemma checkFresh01 : fresh 0 1 = 2.
+Proof. reflexivity. Qed.
+
+Lemma checkFresh02 : fresh 0 2 = 1.
+Proof. reflexivity. Qed.
+
+Lemma checkFresh10 : fresh 1 0 = 2.
+Proof. reflexivity. Qed.
+
+Lemma checkFresh11 : fresh 1 1 = 0.
+Proof. reflexivity. Qed.
+
+Lemma checkFresh12 : fresh 1 2 = 0.
+Proof. reflexivity. Qed.
+
+Lemma checkFresh22 : fresh 2 2 = 0.
+Proof. reflexivity. Qed.
 
