coq/ref/CIC.v
@@ -21,43 +21,70 @@ Inductive isSort : Exp -> Prop :=
 | SortType : forall (n:nat), isSort (EType n)
 .
 
-(* Type for 'local declaration'                                                 *)
+(* Type for 'local declarations' of 'variables'                                 *)
 Inductive LocalDecl : Type :=
 | LAssume : nat -> Exp -> LocalDecl         (* n:T , T is a type                *)
 | LDefine : nat -> Exp -> Exp -> LocalDecl  (* n := (t:T)                       *)
 .
 
-(* Returns variable involved in given local declaration.                        *)
-Definition declVar (decl:LocalDecl) : nat :=
-    match decl with
-    | LAssume n _   => n
-    | LDefine n _ _ => n
-    end.
-
 (* Variable involved must be distinct                                           *)
 Definition LocalContext : Type := list LocalDecl. 
 
-Definition inLocCtx (n:nat) (C:LocalContext) : Prop := 
-    In n (map declVar C).
+(* Whether a variable n is declared in the local context C.                     *)
+Fixpoint inCtxVar (n:nat) (C:LocalContext) : Prop :=
+    match C with
+    | []        => False
+    | d :: C'   =>
+        match d with
+        | LAssume m _   => (n = m) \/ inCtxVar n C'
+        | LDefine m _ _ => (n = m) \/ inCtxVar n C'
+        end
+    end.
 
+(* Whether a declaration is present in the local context C.                     *)
+Fixpoint inCtxDecl (n:nat) (T:Exp) (C:LocalContext) : Prop :=
+    match C with
+    | []        => False
+    | d :: C'   =>
+        match d with
+        | LAssume n' T'     => ((n = n') /\ (T = T')) \/ inCtxDecl n T C'
+        | LDefine n' _ T'   => ((n = n') /\ (T = T')) \/ inCtxDecl n T C'
+        end
+    end.
+
+(* Type for 'global declarations' of 'constants'                                *)
 Inductive GlobalDecl : Type :=
 | GAssume : nat -> Exp -> GlobalDecl        (* c:T, T is a type                 *)
 | GDefine : nat -> Exp -> Exp -> GlobalDecl (* c := t : T                       *)
 | GInduct : nat -> GlobalDecl               (* TBT, define inductive objects    *)
 .
  
-(* Returns constant involved in given global declaration.                       *)
-Definition declConst (decl:GlobalDecl) : nat :=
-    match decl with
-    | GAssume n _   => n
-    | GDefine n _ _ => n
-    | GInduct n     => n
-    end.
-
 Definition GlobalEnv : Type := list GlobalDecl.
 
-Definition inGblEnv (n:nat) (E:GlobalEnv) : Prop := 
-    In n (map declConst E).
+(* Whether a constant n is declared in the global environment E.                *)
+Fixpoint inEnvConst (n:nat) (E:GlobalEnv) : Prop :=
+    match E with
+    | []        => False
+    | d :: E'   =>
+        match d with
+        | GAssume m _   => (n = m) \/ inEnvConst n E'
+        | GDefine m _ _ => (n = m) \/ inEnvConst n E'
+        | GInduct m     => (n = m) \/ inEnvConst n E'
+        end
+    end.
+
+(* Whether a declaration is present in the global environment E.                *)
+Fixpoint inEnvDecl (n:nat) (T:Exp) (E:GlobalEnv) : Prop :=
+    match E with
+    | []        => False
+    | d :: E'   =>
+        match d with
+        | GAssume n' T'     => ((n = n') /\ (T = T')) \/ inEnvDecl n T E'
+        | GDefine n' _ T'   => ((n = n') /\ (T = T')) \/ inEnvDecl n T E'
+        | GInduct _         => inEnvDecl n T E'
+        end
+    end.
+
 
 (* Judgement: E[C] |- t:T                                                       *)
 (* t is well-typed and has type T in the global env E and local context C       *)
@@ -70,34 +97,59 @@ Definition inGblEnv (n:nat) (E:GlobalEnv) : Prop :=
 
 Inductive Entails : GlobalEnv -> LocalContext -> Exp -> Exp -> Prop :=
 | AxProp: forall E C,
-    WF E C                      ->          (* WF(E)[C]                         *)
-    Entails E C EProp (EType 1)             (* E[C] |- Prop:Type(1)             *)
+    WF E C                                  ->  (* WF(E)[C]                     *)
+    Entails E C EProp (EType 1)                 (* E[C] |- Prop:Type(1)         *)
 | AxSet: forall E C,
-    WF E C                      ->          (* WF(E)[C]                         *)
-    Entails E C ESet (EType 1)              (* E[C] |- Set:Type(1)              *)
+    WF E C                                  ->  (* WF(E)[C]                     *)
+    Entails E C ESet (EType 1)                  (* E[C] |- Set:Type(1)          *)
 | AxType: forall E C n,
-    WF E C                      ->          (* WF(E)[C]                         *)
-    Entails E C (EType n) (EType (S n))     (* E[C] |- Type(n):Type(n+1)        *)
+    WF E C                                  ->  (* WF(E)[C]                     *)
+    Entails E C (EType n) (EType (S n))         (* E[C] |- Type(n):Type(n+1)    *)
+| Var: forall E C T n,
+    WF E C                                  ->  (* WF(E)[C]                     *)
+    inCtxDecl n T C                         ->  (* n:T or n := t:T (some t) in C*)
+    Entails E C (EVar n) T                      (* E[C] |- n:T                  *)
+| Con: forall E C T n,
+    WF E C                                  ->  (* WF(E)[C]                     *)
+    inEnvDecl n T E                         ->  (* n:T or n := t:T (some t) in E*)
+    Entails E C (ECon n) T                      (* E[C] |- n:T                  *)
+| ProdProp: forall E C T s n U,
+    Entails E C T s                         ->  (* E[C] |- T:s                  *)
+    isSort s                                ->  (* s is Prop, Set or Type(n)    *)
+    Entails E ((LAssume n T) :: C) U EProp  ->  (* E[(n:T) :: C] |- U:Prop      *)
+    Entails E C (EProd n T U) EProp             (* E[C] |- A(n:T),U  :Prop      *)
+| ProdSet: forall E C T s n U,
+    Entails E C T s                         ->  (* E[C] |- T:s                  *)
+    (s = EProp \/ s = ESet)                 ->  (* s is Prop or Set             *)
+    Entails E ((LAssume n T) :: C) U ESet   ->  (* E[(n:T) :: C] |- U:Set       *)
+    Entails E C (EProd n T U) ESet              (* E[C] |- A(n:T),U  :Set       *)
+| ProdType: forall E C T i n U,
+    Entails E C T (EType i)                 ->  (* E[C] |- T:Type(i)            *)
+    Entails E ((LAssume n T)::C) U (EType i)->  (* E[(n:T) :: C] |- U:Type(i)   *)
+    Entails E C (EProd n T U) (EType i)         (* E[C] |- A(n:T),U  :Set       *)
+| Lam: forall E C n T U s t,
+    Entails E C (EProd n T U) s             ->
+    Entails E ((LAssume n T)::C) t U        ->
+    Entails E C (ELam n T t) (EProd n T U)
 with WF : GlobalEnv -> LocalContext -> Prop :=  
 | WEmpty: WF [] []
 | WLocalAssume: forall E C T s n, 
-    Entails E C T s             ->          (* E[C] |- T:s                      *)
-    isSort s                    ->          (* s is Prop, Set or Type(n)        *) 
-    ~ inLocCtx n C              ->          (* Var n not already in C           *)
-    WF E ((LAssume n T) :: C)               (* WF(E)[ (n:T) :: C]               *) 
+    Entails E C T s                         ->  (* E[C] |- T:s                  *)
+    isSort s                                ->  (* s is Prop, Set or Type(n)    *) 
+    ~ inCtxVar n C                          ->  (* Var n not already in C       *)
+    WF E ((LAssume n T) :: C)                   (* WF(E)[ (n:T) :: C]           *) 
 | WLocalDef: forall E C t T n,
-    Entails E C t T             ->          (* E[C] |- t:T                      *)
-    ~ inLocCtx n C              ->          (* Var n not already in C           *)
-    WF E ((LDefine n t T) :: C)             (* WF(E)[ (n := t:T) :: C ]         *)
+    Entails E C t T                         ->  (* E[C] |- t:T                  *)
+    ~ inCtxVar n C                          ->  (* Var n not already in C       *)
+    WF E ((LDefine n t T) :: C)                 (* WF(E)[ (n := t:T) :: C ]     *)
 | WGlobalAssume: forall E T s n,         
-    Entails E [] T s            ->          (* E[[]] |- T:s                     *)
-    isSort s                    ->          (* s is Prop, Set or Type(n)        *)
-    ~ inGblEnv n E              ->          (* Const n not already in E         *)
-    WF ((GAssume n T) :: E) []              (* WF((n:T) :: E)[]                 *)
+    Entails E [] T s                        ->  (* E[[]] |- T:s                 *)
+    isSort s                                ->  (* s is Prop, Set or Type(n)    *)
+    ~ inEnvConst n E                        ->  (* Const n not already in E     *)
+    WF ((GAssume n T) :: E) []                  (* WF((n:T) :: E)[]             *)
 | WGlobalDef: forall E t T n,
-    Entails E [] t T            ->          (* E[[]] |- t:T                     *)
-    ~ inGblEnv n E              ->          (* Const n not already in E         *)
-    WF ((GDefine n t T) :: E) []            (* WF((n := t:T) :: E)[]            *)                           
+    Entails E [] t T                        ->  (* E[[]] |- t:T                 *)
+    ~ inEnvConst n E                        ->  (* Const n not already in E     *)
+    WF ((GDefine n t T) :: E) []                (* WF((n := t:T) :: E)[]        *)                           
 .
-
 
