agda/plfa/bin.agda
@@ -1,8 +1,10 @@
 module bin where
 
-open import nat
-open import plus
-open import mult
+import Relation.Binary.PropositionalEquality as Eq
+open Eq using (_≡_; refl; cong; sym)
+open Eq.≡-Reasoning using (begin_; _≡⟨⟩_; _≡⟨_⟩_;_∎)
+open import Data.Nat using (ℕ; zero; suc; _+_; _*_; _∸_;_^_) -- \.-
+
 
 data Bin : Set where
   ⟨⟩ : Bin
@@ -28,12 +30,25 @@ b4 = inc b₂
 
 to : ℕ → Bin
 to  zero = ⟨⟩ O
-to (succ n) = inc (to n)
+to (suc n) = inc (to n)
 
 from : Bin → ℕ
 from ⟨⟩    = 0
 from (n O) = 2 * (from n)
 from (n I) = 2 * (from n) + 1
+
+from-inc : ∀ (b : Bin) → from (inc b) ≡ suc (from b)
+from-inc ⟨⟩ = refl
+from-inc (b O) =
+  begin
+    from (inc (b O))
+    ≡⟨⟩
+    from (b I)
+    ≡⟨⟩
+    2 * (from b) + 1
+    ≡⟨⟩
+    {!!}
+from-inc (b I) = {!!}
 
 
 
